src/ssa/extraction/ssa_main.ml
@@ -1,0 +1,40 @@
+open Ssa_interpreter
+open Ssa_dynamic
+open Printf
+open Llvm
+open Llvm_executionengine
+
+let main in_filename  =
+
+
+        let ic = create_context () in
+        let imbuf = MemoryBuffer.of_file in_filename in
+        let im = Llvm_bitreader.parse_bitcode ic imbuf in
+        let ist = SlotTracker.create_of_module im in
+        let imp = ModuleProvider.create im in
+
+        dump_module im;
+        Llvm_pretty_printer.travel_module ist im;
+        let coqim = Translator.translate_module ist im in
+        Coq_pretty_printer.travel_module coqim;
+
+        let li = ExecutionEngine.create_interpreter imp in
+
+        (match LLVMopsem.ds_genInitState (coqim::[]) "main" [] (li, im) with
+          | Some s ->
+            (match interInsn s with
+              | Some (s', tr) -> ()
+              | None -> () )
+          | None -> () );
+
+        SlotTracker.dispose ist;
+        ExecutionEngine.dispose li;
+        ModuleProvider.dispose imp
+
+let () = match Sys.argv with
+        | [| _; in_filename |] -> main in_filename
+        | _ -> main "Input.bc"
+
+
+
+
