src/TV/seop_llvmop.v
@@ -2,7 +2,8 @@ Add LoadPath "../ssa/ott".
 Add LoadPath "../ssa/monads".
 Add LoadPath "../ssa".
 (*Add LoadPath "../../../theory/metatheory".*)
-Require Import ssa.
+Require Import ssa_def.
+Require Import ssa_lib.
 Require Import List.
 Require Export targetdata.
 Require Import monad.
